cedar-dafny/pe/engine.dfy
@@ -3,6 +3,7 @@ include "../def/std.dfy"
 include "../def/base.dfy"
 include "../def/core.dfy"
 include "../def/engine.dfy"
+include "environment.dfy"
 
 module pe.engine {
   import opened definition
@@ -10,6 +11,7 @@ module pe.engine {
   import opened def.base
   import opened def.core
   import opened def.engine
+  import opened environment
 
   datatype PartialEvaluator = PartialEvaluator(request: definition.Request, store: definition.EntityStore) {
 
@@ -18,9 +20,9 @@ module pe.engine {
         case PrimitiveLit(p) => Ok(Concrete(Primitive(p)))
         case Var(v) =>
           match v {
-            case Principal => Ok(Residual.fromOptionalEntity(request.principal))
-            case Action => Ok(Residual.fromOptionalEntity(request.action))
-            case Resource => Ok(Residual.fromOptionalEntity(request.resource))
+            case Principal => Ok(Residual.fromRequestEntity(request.principal))
+            case Action => Ok(Residual.fromRequestEntity(request.action))
+            case Resource => Ok(Residual.fromRequestEntity(request.resource))
             case Context => Ok(Residual.fromRecord(request.context))
           }
         case If(e_cond, e_true, e_false) =>
@@ -29,50 +31,135 @@ module pe.engine {
             case Concrete(v) =>
               var b_cond :- Value.asBool(v);
               if b_cond then interpret(e_true) else interpret(e_false)
-            case _ => Err(TypeError)
+            case _ =>
+              match (interpret(e_true), interpret(e_false)) {
+                // ignore the error of the else branch
+                case (Err(err1), Err(_)) => Err(err1)
+                case (Ok(Concrete(v1)), Ok(Concrete(v2))) => Ok(Residual.If(v_cond, Concrete(v1), Concrete(v2)))
+                case (Ok(Concrete(v1)), Ok(r2)) => Ok(Residual.If(v_cond, Concrete(v1), r2))
+                case (Ok(r1), Ok(Concrete(v2))) => Ok(Residual.If(v_cond, r1, Concrete(v2)))
+                case (Ok(r1), Ok(r2)) => Ok(Residual.If(v_cond, r1, r2))
+                case (Err(_), Ok(r2)) => Ok(Residual.If(v_cond, makeErrorValue(), r2))
+                case (Ok(r1), Err(_)) => Ok(Residual.If(v_cond, r1, makeErrorValue()))
+              }
           }
         case BinaryApp(op, e1, e2) =>
           var r1 :- interpret(e1);
           var r2 :- interpret(e2);
           match (r1, r2) {
-            case (Concrete(v1), Concrete(v2)) => Err(TypeError)
-            case _ => Err(TypeError)
+            case (Concrete(v1), Concrete(v2)) => Evaluator.applyBinaryOpGeneric(op, v1, v2, store).Map(v => Concrete(v))
+            case (Concrete(v), _) => Ok(Residual.BinaryApp(op, Concrete(v), r2))
+            case (_, Concrete(v)) => Ok(Residual.BinaryApp(op, r1, Concrete(v)))
+            case _ => Ok(Residual.BinaryApp(op, r1, r2))
           }
         case UnaryApp(op, e) =>
           var r :- interpret(e);
           match r {
             case Concrete(v) =>
-              var cv :- engine.Evaluator.applyUnaryOp(op, v);
+              var cv :- Evaluator.applyUnaryOp(op, v);
               Ok(Concrete(cv))
             case _ => Ok(Residual.UnaryApp(op, r))
           }
         case GetAttr(e, a) =>
           var r :- interpret(e);
-          Err(TypeError)
+          match r {
+            case Concrete(v) =>
+              if v.Record? then
+                if a in v.record.Keys then Ok(Concrete(v.record[a])) else Err(AttrDoesNotExist)
+              else
+                var uid :- Value.asEntity(v);
+                var res :- store.getEntityAttrs(uid);
+                if a in res.Keys then Ok(res[a]) else Err(AttrDoesNotExist)
+            case _ => Ok(Residual.GetAttr(r, a))
+          }
         case HasAttr(e, a) =>
           var r :- interpret(e);
-          Err(TypeError)
+          match r {
+            case Concrete(v) =>
+              if v.Record? then
+                Ok(Concrete(Value.Bool(a in v.record.Keys)))
+              else
+                var uid :- Value.asEntity(v);
+                var res :- store.getEntityAttrs(uid);
+                Ok(Concrete(Value.Bool(a in res.Keys)))
+            case _ => Ok(Residual.GetAttr(r, a))
+          }
         case Set(es) =>
-          var rs :- interpretSet(es);
-          Ok(splitSeq(rs))
+          var rs :- interpretSeq(es);
+          Ok(splitSeqToSet(rs))
         case Record(bs) =>
           var rs :- interpretRecord(bs);
           Ok(splitRecord(rs))
         case Unknown(u) => Ok(Residual.Unknown(u))
-        case _ => Err(TypeError)
+        case And(e1, e2) =>
+          var l :- interpret(e1);
+          match l {
+            case Concrete(v1) =>
+              var b :- Value.asBool(v1);
+              if !b
+              then Ok(l)
+              else
+                var r :- interpret(e2);
+                match r {
+                  case Concrete(v2) =>
+                    Value.asBool(v2).Map(v => Concrete(v2))
+                  case _ => Ok(Residual.And(l, r))
+                }
+            case _ =>
+              var rr := interpret(e2);
+              Ok(Residual.And(l, match rr {
+                                case Ok(r) =>
+                                  r
+                                case _ => makeErrorValue()
+                              }))
+          }
+        case Or(e1, e2) =>
+          var l :- interpret(e1);
+          match l {
+            case Concrete(v1) =>
+              var b :- Value.asBool(v1);
+              if b
+              then Ok(l)
+              else
+                var r :- interpret(e2);
+                match r {
+                  case Concrete(v2) =>
+                    Value.asBool(v2).Map(v => Concrete(v2))
+                  case _ => Ok(Residual.Or(l, r))
+                }
+            case _ =>
+              var rr := interpret(e2);
+              Ok(Residual.Or(l, match rr {
+                               case Ok(r) =>
+                                 r
+                               case _ => makeErrorValue()
+                             }))
+          }
+        case Call(fn, args) =>
+          var rs :- interpretSeq(args);
+          if (forall r | r in rs :: r.Concrete?) then
+            Evaluator.applyExtFun(fn, seq(|rs|, i requires 0 <= i < |rs| => rs[i].v)).Map(v => Concrete(v))
+          else
+            Ok(Residual.Call(fn, rs))
       }
     }
 
-    function interpretSet(es: seq<definition.Expr>): definition.Result<seq<Residual>> {
+    function makeErrorValue(): (r : Residual)
+      ensures forall env : Environment :: env.wellFormed() ==> env.interpret(r).Err?
+    {
+      Residual.GetAttr(Residual.Record([]), "")
+    }
+
+    function interpretSeq(es: seq<definition.Expr>): definition.Result<seq<Residual>> {
       if |es| == 0 then
         Ok([])
       else
         var r :- interpret(es[0]);
-        var rs :- interpretSet(es[1..]);
+        var rs :- interpretSeq(es[1..]);
         Ok([r] + rs)
     }
 
-    function splitSeq(rs: seq<Residual>): Residual {
+    function splitSeqToSet(rs: seq<Residual>): Residual {
       if (forall r | r in rs :: r.Concrete?) then
         Concrete(Value.Set(set x | x in rs :: x.v))
       else
